examples/l3-machine-code/lib/FP32.sml
@@ -4,10 +4,19 @@
 
 structure FP32 :> FP =
 struct
+
+   type ieee_flags = {DivideByZero: bool,
+                      InvalidOp: bool,
+                      Overflow: bool,
+                      Precision: bool,
+                      Underflow: bool}
+
    val posInf = BitsN.BV (0, 0)
    val negInf = BitsN.BV (0, 0)
    val posZero = BitsN.BV (0, 0)
    val negZero = BitsN.BV (0, 0)
+   val sNan = BitsN.BV (0, 0)
+   val qNan = BitsN.BV (0, 0)
 
    fun err s = raise Fail (s ^ ": not supported")
 
@@ -17,8 +26,10 @@ struct
 
    fun isFinite _ = err "isFinite"
    fun isNan _ = err "isNan"
+   fun isSignallingNan _ = err "isSignallingNan"
    fun isNormal _ = err "isNormal"
    fun isSubnormal _ = err "isSubnormal"
+   fun isIntegral _ = err "isIntegral"
    fun abs _ = err "abs"
    fun neg _ = err "neg"
    fun add _ = err "add"
@@ -34,5 +45,6 @@ struct
    fun greaterEqual _ = err "greaterEqual"
    fun lessThan _ = err "lessThan"
    fun lessEqual _ = err "lessEqual"
+   fun roundToIntegral _ = err "lessEqual"
 
 end (* structure FP32 *)
